Working on the tactics. Reorganising some files.

lib/extra/Array.v
@@ -14,12 +14,30 @@ Parameter array : Type -> Type.
 
 Parameter length : forall T, array T -> nat.
 
+Parameter read_option : forall T, array T -> nat -> option T.
 Parameter read : forall T `{Inhab T}, array T -> nat -> T.
 Parameter write : forall T, array T -> nat -> T -> array T.
 
 Parameter empty : forall T, array T.
 Parameter from_list : forall T, list T -> array T.
 Parameter to_list : forall T, array T -> list T.
+
+Parameter read_option_Some : forall T `{Inhab T} a n,
+  n < length a ->
+  read_option a n = Some (read a n).
+
+Parameter read_option_None : forall T (a : array T) n,
+  n >= length a ->
+  read_option a n = None.
+
+Parameter read_option_write_eq : forall T a (t : T) n,
+  n < length a ->
+  read_option (write a n t) n = Some t.
+
+Parameter read_option_write_neq : forall T a (t : T) n1 n2,
+  n2 < length a ->
+  n1 <> n2 ->
+  read_option (write a n1 t) n2 = read_option a n2.
 
 Parameter read_write_eq : forall T `{Inhab T} a (t : T) n,
   n < length a ->
@@ -41,6 +59,12 @@ Parameter from_list_length : forall T (l : list T),
 
 Parameter to_list_length : forall T (a : array T),
   LibList.length (to_list a) = length a.
+
+Parameter from_list_read_option : forall T (l : list T) n,
+  read_option (from_list l) n = nth_option n l.
+
+Parameter to_list_read_option : forall T (a : array T) n,
+  nth_option n (to_list a) = read_option a n.
 
 Parameter from_list_read : forall T `{Inhab T} (l : list T) n,
   read (from_list l) n = nth n l.
@@ -75,6 +99,7 @@ Definition array := list.
 
 Definition length T := length : array T -> nat.
 
+Definition read_option T (a : array T) n := nth_option n a.
 Definition read T `{Inhab T} (a : array T) n := nth n a.
 Definition write T (a : array T) n t := update n t a : array T.
 
@@ -83,6 +108,31 @@ Definition to_list T := id : array T -> list T.
 
 Definition empty T := from_list nil : array T.
 Arguments empty [T].
+
+Lemma read_option_Some : forall T `{Inhab T} a n,
+  n < length a ->
+  read_option a n = Some (read a n).
+Proof. introv I. apply~ nth_option_Some. Qed.
+
+Lemma read_option_None : forall T (a : array T) n,
+  n >= length a ->
+  read_option a n = None.
+Proof. introv I. apply~ nth_option_length. Qed.
+
+Lemma read_option_write_eq : forall T a (t : T) n,
+  n < length a ->
+  read_option (write a n t) n = Some t.
+Proof. introv I. apply~ nth_option_update_eq. Qed.
+
+Lemma read_option_write_neq : forall T a (t : T) n1 n2,
+  n2 < length a ->
+  n1 <> n2 ->
+  read_option (write a n1 t) n2 = read_option a n2.
+Proof.
+  introv I D. tests I': (n1 < length a).
+   apply~ nth_option_update_neq.
+   unfolds write. rewrite~ update_out. unfolds length. nat_math.
+Qed.
 
 Lemma read_write_eq : forall T `{Inhab T} a (t : T) n,
   n < length a ->
@@ -109,6 +159,14 @@ Proof. reflexivity. Qed.
 
 Lemma empty_length : forall T,
   length (@empty T) = 0.
+Proof. reflexivity. Qed.
+
+Lemma from_list_read_option : forall T (l : list T) n,
+  read_option (from_list l) n = nth_option n l.
+Proof. reflexivity. Qed.
+
+Lemma to_list_read_option : forall T (a : array T) n,
+  nth_option n (to_list a) = read_option a n.
 Proof. reflexivity. Qed.
 
 Lemma from_list_read : forall T `{Inhab T} (l : list T) n,
