low/Relation.v
@@ -2,7 +2,7 @@
  * Relation between the low-level formalisation to the C source code of R. **)
 
 Set Implicit Arguments.
-Require Export Rinvariants.
+Require Export Invariants.
 
 (* TODO *)
 
